code/ecdsa/Hacl.Impl.EC.P521.Reduction.fst
@@ -9,38 +9,106 @@ open FStar.Math.Lemmas
 open FStar.Math.Lib
 open Lib.Buffer
 
-open Hacl.SolinasReduction.Lemmas
 open Hacl.Impl.P256.LowLevel 
 
 open Spec.P256
 open Hacl.Spec.P256.Definition
 open FStar.Mul
 
-open Hacl.Impl.EC.MontgomeryMultiplication
+open Hacl.Impl.EC.MontgomeryMultiplication.Lemmas
+
+#set-options " --z3rlimit 200" 
 
 
 let coordinate521 = 9ul
 let prime521 = pow2 521 - 1
 
-assume val lemma_test: #l: size_nat -> c: curve ->  a: Lib.Sequence.lseq uint64 l -> i: nat {i <= l} -> 
-  Lemma (ensures (
-    let a0 = Lib.Sequence.sub a 0 i in 
-    let a1 = Lib.Sequence.sub a i (l - i) in 
-    lseq_as_nat a = lseq_as_nat a0 + pow2 (64 * i) * lseq_as_nat a1))
-    (decreases (l - i))
+let felem = lbuffer uint64 (coordinate521)
+let widefelem = lbuffer uint64 (coordinate521 *. 2ul)
+
+assume val felem_add: a: felem -> b: felem -> out: felem ->  Stack unit
+    (requires (fun h -> 
+      live h a /\ live h b /\ live h out /\ eq_or_disjoint a out /\  eq_or_disjoint b out /\
+      lseq_as_nat (as_seq h a) < prime521 /\ lseq_as_nat (as_seq h b) < prime521))
+    (ensures (fun h0 _ h1 -> 
+      modifies (loc out) h0 h1 /\ 
+      lseq_as_nat (as_seq h1 out) == (lseq_as_nat (as_seq h0 a) + lseq_as_nat (as_seq h1 b)) % prime521))
 
 
-val reduction_p521: i: lbuffer uint64 (coordinate521 *. 2ul) -> o: lbuffer uint64 coordinate521 -> 
+assume val reduction_prime_2prime:  x: felem-> result: felem -> 
   Stack unit
-    (requires fun h -> live h i /\ live h o /\ disjoint i o /\ lseq_as_nat (as_seq h i) < prime521 * prime521)
+    (requires fun h -> 
+      live h x /\ live h result /\ eq_or_disjoint x result)
+    (ensures fun h0 _ h1 -> 
+      modifies (loc result) h0 h1 /\ lseq_as_nat (as_seq h1 result) == lseq_as_nat (as_seq h0 x) % prime521)
+
+
+
+val lemma_second_word_reduction: t0: Lib.Sequence.lseq uint64 (v coordinate521) -> t1: Lib.Sequence.lseq uint64 (v coordinate521) -> 
+  Lemma 
+    (requires (lseq_as_nat t0 + pow2 (64 * v coordinate521) * lseq_as_nat t1 < prime521 * pow2 (64 * v coordinate521)))
+    (ensures(lseq_as_nat t1 < prime521))
+
+
+let lemma_second_word_reduction t0 t1 = 
+  lseq_upperbound t0;
+  assert(lseq_as_nat t1 < prime521)
+
+
+val getZeroWord: i: widefelem -> o: felem -> Stack unit
+  (requires fun h -> live h i /\ live h o /\ disjoint i o)
+  (ensures fun h0 _ h1 -> modifies (loc o) h0 h1)
+
+let getZeroWord i o = 
+  copy o (sub i (size 0) (size 9));
+  let o8 = index o (size 8) in 
+  let o8Updated = logand (u64 0x00000000000002ff) o8 in 
+  upd o (size 8) o8Updated
+  
+  (* 576 bits copies *)
+
+
+val getFirstWord: i: widefelem -> o: felem -> Stack unit 
+  (requires fun h -> True)
+  (ensures fun h0 _ h1 -> True)
+
+let getFirstWord i o = 
+  let flag0 = u64 0xfffffffffffffd00 in 
+  let flag1 = u64 0x00000000000002ff in 
+  let i0 = index i (size 9) in 
+  let i1 = index i (size 10) in 
+
+  let i0_ = logand i0 flag0 in 
+  let i1_ = logand i1 flag1 in 
+
+  let o0 = logxor i0_ i1_ in 
+  upd o (size 0) o0
+
+
+
+val reduction_p521: i: widefelem -> o: felem -> 
+  Stack unit
+    (requires fun h -> live h i /\ live h o /\ disjoint i o /\ lseq_as_nat (as_seq h i) < prime521 * pow2 (64 * v coordinate521))
     (ensures fun h0 _ h1 -> modifies1 o h0 h1 /\ 
-      lseq_as_nat (as_seq h0 i) % prime521 == lseq_as_nat (as_seq h1 i))
+      lseq_as_nat (as_seq h0 i) % prime521 == lseq_as_nat (as_seq h1 o))
 
 let reduction_p521 i o = 
-  let t0 = sub i (size 0) coordinate521 in 
-  let t1 = sub i coordinate521 coordinate521 in 
+  push_frame();
+    let a0 = create (size 9) (u64 0) in 
+    let a1 = create (size 9) (u64 0) in 
+    let a2 = create (size 9) (u64 0) in 
 
-  lemma_test 
+  getZeroWord i a0;
+  getFirstWord i a1;
+  getFirstWord i a2;
+  
+
+
+
+
+  felem_add a0 a1 o;
+  felem_add o a2 o;
+
 
   admit()
 
